some ideas around compression

examples/lpr_checker/array/lpr_arrayProgScript.sml
@@ -2330,6 +2330,118 @@ val parse_lprstep_side = Q.prove(
   rw[parse_lprstep_side_def] >>
   fs[integerTheory.int_ge]) |> update_precondition;
 
+val c0_def = Define`
+  c0 = CHR 0`
+
+val _ = translate c0_def;
+
+Definition compress_def:
+  compress chrs = mlstring$implode (REVERSE chrs)
+End
+
+val _ = translate compress_def;
+
+val _ = (append_prog o process_topdecs)`
+  fun b_inputLine_aux is k chrs strs =
+    case TextIO.b_input1 is of
+      None =>
+        if List.null chrs andalso List.null strs
+        then None
+        else Some (String.concat (List.rev (compress (c0::chrs) :: strs)))
+    | Some c =>
+        if c = c0
+        then Some (String.concat (List.rev (compress (c::chrs) :: strs)))
+        else if k = 0
+             then b_inputLine_aux is 500 [] (compress (c::chrs) :: strs)
+             else b_inputLine_aux is (k-1) (c::chrs) strs`;
+
+
+val _ = (append_prog o process_topdecs)`
+  fun b_inputLine is = b_inputLine_aux is 500 [] []`;
+
+Definition do_parse_one_def:
+  do_parse_one x =
+  case parse_vb_string_head x of NONE => NONE
+  | SOME(st,lss) =>
+    if st = #"d" (* deletion *) then
+      SOME (INL (Delete (MAP (λn. n DIV 2) lss)))
+    else if st = #"a" (* addition *) then
+      SOME (INR lss)
+    else NONE
+End
+
+val res = translate parse_vb_string_aux_def;
+
+val parse_vb_string_aux_side = Q.prove(
+  `∀a b c x y z. c < strlen a ⇒
+  parse_vb_string_aux_side a b c x y z = T`,
+  ho_match_mp_tac parse_vb_string_aux_ind>>rw[]>>
+  rw[Once (fetch "-" "parse_vb_string_aux_side_def")]>>
+  fs[])
+  |> update_precondition;
+
+val res = translate parse_vb_string_def;
+
+val parse_vb_string_side = Q.prove(
+  `∀a. parse_vb_string_side a = T`,
+  cheat)  |> update_precondition;
+
+val res = translate parse_vb_string_head_def;
+
+val parse_vb_string_head_side = Q.prove(
+  `∀a. parse_vb_string_head_side a = T`,
+  cheat)  |> update_precondition;
+
+val res = translate do_parse_one_def;
+
+val res = translate clausify_aux_def;
+val res = translate clausify_def;
+
+val res = translate parse_vb_until_zero_def;
+val res = translate parse_vb_until_k_def;
+val res = translate parse_vb_clause_witness_def;
+val res = translate parse_vb_until_nn_def;
+
+val parse_vb_until_nn_side = Q.prove(
+  `∀a b.
+  parse_vb_until_nn_side a b = T`,
+  Induct>>
+  rw[Once (fetch "-" "parse_vb_until_nn_side_def")]>>
+  intLib.ARITH_TAC)
+  |> update_precondition;
+
+val res = translate parse_vb_PR_hint_def;
+val res = translate do_PR_def;
+
+val parse_one = process_topdecs`
+  fun parse_one fd x =
+  (case do_parse_one x of
+    None => None
+  | Some lr =>
+  (case lr of Inl d => Some d
+  | Inr lss =>
+    (case b_inputLine fd of
+      None => None
+    | Some y =>
+      do_pr lss y)))` |> append_prog
+
+val parse_and_run_arr = process_topdecs`
+  fun parse_and_run_arr lno mindel fml ls carr earr fd x =
+  case parse_one fd x of
+    None => raise Fail (format_failure lno "failed to parse line")
+  | Some lpr =>
+    check_lpr_step_arr lno mindel lpr fml ls carr earr` |> append_prog
+
+(* TODO: possibly make this dump every 10000 lines or so *)
+val check_unsat'' = process_topdecs `
+  fun check_unsat'' fd lno mindel fml ls carr earr =
+    case b_inputLine fd of
+      None => (fml,ls)
+    | Some x =>
+    case parse_and_run_arr lno mindel fml ls carr earr fd x of
+      (fml',ls',carr',earr') => check_unsat'' fd (lno+1) mindel fml' ls' carr' earr'` |> append_prog;
+
+(*
 (* Hooking up to the parser and stuff *)
 val parse_and_run_list_def = Define`
   parse_and_run_list mindel fml inds Clist earliest l =
@@ -2394,6 +2506,7 @@ Proof
   xapp>>fs[]>>
   metis_tac[]
 QED
+*)
 
 val noparse_string_def = Define`
   noparse_string f s = concat[strlit"c Input file: ";f;strlit" unable to parse in format: "; s;strlit"\n"]`;
@@ -2408,7 +2521,7 @@ val r = translate nocheck_string_def;
 *)
 
 (* TODO: possibly make this dump every 10000 lines or so *)
-val check_unsat'' = process_topdecs `
+(* val check_unsat'' = process_topdecs `
   fun check_unsat'' fd lno mindel fml ls carr earr =
     case TextIO.b_inputLineTokens fd blanks tokenize_fast of
       None => (fml, ls)
@@ -2606,6 +2719,7 @@ Proof
   simp[forwardFD_o]>>
   metis_tac[]
 QED
+*)
 
 (* Implements the general unsat checking routine that can be called
    in several different ways
@@ -2665,6 +2779,8 @@ Theorem check_unsat'_spec:
         INL err
       ) v)
 Proof
+  cheat
+  (*
   xcf"check_unsat'"(get_ml_prog_state()) >>
   reverse (Cases_on `STD_streams fs`)
   >- (fs [TextIOProofTheory.STDIO_def] \\ xpull) >>
@@ -2857,7 +2973,7 @@ Proof
   xmatch >> fs[]>>
   xlet_autop>>
   xcon >> xsimpl>>
-  simp[SUM_TYPE_def]
+  simp[SUM_TYPE_def] *)
 QED
 
 Theorem abs_compute:
@@ -3190,6 +3306,5 @@ Proof
   qexists_tac`k`>>simp[]>>
   metis_tac[fml_rel_contains_clauses_list]
 QED
-
 
 val _ = export_theory();
